src/Equality.v
@@ -4,4 +4,7 @@ Class Eq
      ; eq_refl: forall t: T, eq t t
      ; eq_sym: forall t t': T, eq t t' -> eq t' t
      ; eq_trans: forall t t' t'': T, eq t t' -> eq t' t'' -> eq t t''
-     ; eq_dec: forall t t': T, {eq t t'} + {~ eq t t'} }.
+     ; eq_dec: forall t t': T, {eq t t'} + {~ eq t t'}
+     ; eq_equal: forall t t': T, eq t t' -> t = t'
+     ; equal_eq: forall t t': T, t = t' -> eq t t'
+     }.
